src/program_proof/wal/common_proof.v
@@ -38,7 +38,6 @@ Proof.
   iApply "HΦ".
   iNamed "HmemLog_linv".
   iDestruct "HmemStart_txn" as "#HmemStart_txn".
-  iDestruct "HnextDiskEnd_txn" as "#HnextDiskEnd_txn".
   iDestruct "HmemEnd_txn" as "#HmemEnd_txn".
   iMod (txn_pos_valid_locked with "Hwal HmemEnd_txn Howntxns") as "(%HmemEnd_is_txn & Howntxns)".
   iModIntro.
@@ -47,7 +46,7 @@ Proof.
                        (set slidingM.mutable (λ _ : u64, slidingM.endPos σ.(memLog)) σ.(memLog))) σ).
   simpl.
   iFrame "# ∗".
-  iSplitR "Howntxns HownLoggerPos_linv HownStableSet".
+  iSplitR "Howntxns HownLoggerPos_linv HnextDiskEnd".
   { iExists _; iFrame.
     iPureIntro.
     split_and!; simpl; auto; try word.
@@ -55,7 +54,7 @@ Proof.
     unfold locked_wf, slidingM.wf in Hlocked_wf.
     word.
   }
-  iExists memStart_txn_id, (length txns - 1)%nat, txns, _, _; simpl.
+  iExists memStart_txn_id, (length txns - 1)%nat, txns, _; simpl.
   iFrame "% # ∗".
   destruct_and! His_memLog.
 (*
@@ -69,5 +68,218 @@ Proof.
     now we need to build it from the pieces) *)
 *)
 Admitted.
+
+Lemma is_txn_mid σ (a b c : nat) pos :
+  wal_wf σ ->
+  is_txn σ.(log_state.txns) a pos ->
+  is_txn σ.(log_state.txns) c pos ->
+  a ≤ b ≤ c ->
+  is_txn σ.(log_state.txns) b pos.
+Proof.
+  rewrite /is_txn /wal_wf; intros Hwf Ha Hc Hle.
+  destruct Hwf as [_ [Hwf _]].
+  destruct (decide (a < b)).
+  2: { assert (a = b) by lia; subst; eauto. }
+  destruct (decide (b < c)).
+  2: { assert (b = c) by lia; subst; eauto. }
+  assert (is_Some (σ.(log_state.txns) !! b)).
+  { eapply lookup_lt_is_Some_2. etransitivity.
+    2: {
+      eapply lookup_lt_is_Some_1.
+      eapply fmap_is_Some. eauto.
+    }
+    lia.
+  }
+
+  destruct H as [tb Hb'].
+  assert (fst <$> σ.(log_state.txns) !! b = Some (fst tb)) as Hb.
+  { rewrite Hb'. reflexivity. }
+
+  rewrite -list_lookup_fmap in Ha.
+  rewrite -list_lookup_fmap in Hb.
+  rewrite -list_lookup_fmap in Hc.
+  rewrite -list_lookup_fmap.
+
+  eapply Hwf in Ha as Hab'.
+  1: eapply Hab' in Hb as Hab. 2: lia.
+  eapply Hwf in Hb as Hbc'.
+  1: eapply Hbc' in Hc as Hbc. 2: lia.
+  rewrite Hb. f_equal. word.
+Qed.
+
+Lemma subslice_stable_nils γ σ (txn_id txn_id' : nat) pos :
+  wal_wf σ ->
+  txn_id ≤ txn_id' ->
+  is_txn σ.(log_state.txns) txn_id pos ->
+  is_txn σ.(log_state.txns) txn_id' pos ->
+  ( nextDiskEnd_inv γ σ.(log_state.txns) ∗
+    txn_id [[γ.(stable_txn_ids_name)]]↦ro () ) -∗
+  ⌜Forall (λ x, snd x = nil) (subslice (S txn_id) (S txn_id') σ.(log_state.txns))⌝.
+Proof.
+  intros.
+  iIntros "[Hinv Hstable]".
+  iNamed "Hinv".
+  iDestruct (map_ro_valid with "Hstablectx Hstable") as "%Hvalid".
+  iPureIntro.
+  apply Forall_lookup_2; intros.
+  apply subslice_lookup_some in H3 as H3'.
+  assert (snd <$> σ.(log_state.txns) !! (S txn_id + i)%nat = Some x.2).
+  { rewrite H3'. eauto. }
+  erewrite HafterNextDiskEnd in H4.
+  { congruence. }
+  2: eassumption.
+  { lia. }
+  1: eassumption.
+  eapply is_txn_mid.
+  1: eassumption.
+  1: apply H1.
+  1: apply H2.
+  eapply subslice_lookup_bound' in H3 as Hbound.
+  lia.
+Qed.
+
+Lemma stable_sound_alloc txns stable_txns (txn_id txn_id' : nat) (pos : u64) :
+  stable_txns !! txn_id = Some () ->
+  txn_id ≤ txn_id' ->
+  is_txn txns txn_id pos ->
+  is_txn txns txn_id' pos ->
+  stable_sound txns stable_txns ->
+  stable_sound txns (<[txn_id':=()]> stable_txns).
+Proof.
+  rewrite /stable_sound.
+  intros.
+
+  destruct (decide (txn_id' = txn_id0)).
+  { subst.
+    eapply (H3 txn_id txn_id'0 pos); try eassumption.
+    1: lia.
+    pose proof (is_txn_pos_unique _ _ _ _ H2 H6); subst.
+    eauto.
+  }
+  eapply H3; try eassumption.
+  rewrite lookup_insert_ne in H5; eauto.
+Qed.
+
+Lemma stable_sound_nils σ stable_txns txn_id txn_id' pos :
+  wal_wf σ ->
+  stable_txns !! txn_id = Some () ->
+  is_txn σ.(log_state.txns) txn_id pos ->
+  is_txn σ.(log_state.txns) txn_id' pos ->
+  stable_sound σ.(log_state.txns) stable_txns ->
+  Forall (λ x, x.2 = []) (subslice (S txn_id) (S txn_id') σ.(log_state.txns)).
+Proof.
+  intros.
+  apply Forall_lookup_2; intros.
+  apply subslice_lookup_some in H4 as H4'.
+  assert (snd <$> σ.(log_state.txns) !! (S txn_id + i)%nat = Some x.2).
+  { rewrite H4'. eauto. }
+  erewrite H3 in H5.
+  { congruence. }
+  2: eassumption.
+  { lia. }
+  1: eassumption.
+  eapply is_txn_mid.
+  1: eassumption.
+  1: apply H1.
+  1: apply H2.
+  eapply subslice_lookup_bound' in H4 as Hbound.
+  lia.
+Qed.
+
+Theorem stable_txn_id_advance γ mutable txn_id txn_id' pos nextDiskEnd_txn_id σ :
+  wal_wf σ ->
+  is_txn σ.(log_state.txns) txn_id pos ->
+  is_txn σ.(log_state.txns) txn_id' pos ->
+  txn_id ≤ txn_id' ->
+  memLog_linv_nextDiskEnd_txn_id γ mutable nextDiskEnd_txn_id -∗
+  nextDiskEnd_inv γ σ.(log_state.txns) -∗
+  txn_id [[γ.(stable_txn_ids_name)]]↦ro () -∗
+  txns_ctx γ σ.(log_state.txns)
+  ==∗ (
+    txn_id' [[γ.(stable_txn_ids_name)]]↦ro () ∗
+    nextDiskEnd_inv γ σ.(log_state.txns) ∗
+    txns_ctx γ σ.(log_state.txns) ∗
+    ∃ nextDiskEnd_txn_id',
+      memLog_linv_nextDiskEnd_txn_id γ mutable nextDiskEnd_txn_id' ∗
+      ⌜nextDiskEnd_txn_id ≤ nextDiskEnd_txn_id' < length σ.(log_state.txns)⌝ ∗
+      ⌜Forall (λ x, x.2 = []) (subslice (S nextDiskEnd_txn_id) (S nextDiskEnd_txn_id') σ.(log_state.txns))⌝
+  ).
+Proof.
+  clear P.
+
+  iIntros (Hwf Histxn Histxn' Hle) "H0 H1 #Hstable Htxns_ctx".
+  iNamed "H0".
+  iNamed "H1".
+  iDestruct (map_ctx_agree with "HownStableSet Hstablectx") as "%Heq". subst.
+  iDestruct (map_valid with "HownStableSet Hstable") as "%Hstable".
+
+  iDestruct (map_valid with "Hstablectx HnextDiskEnd_stable") as "%HnextDiskEnd_stable".
+  iDestruct (txn_pos_valid_general with "Htxns_ctx HnextDiskEnd_txn") as "%HnextDiskEnd_txn".
+
+  destruct (stable_txns0 !! txn_id') eqn:He.
+  {
+    iDestruct (big_sepM_lookup with "Hstablero") as "#Hstable'"; eauto.
+    iModIntro.
+    iFrame "Hstable' Htxns_ctx".
+    iSplitL "Hstablectx Hstablero".
+    { iExists _. iFrame. iFrame "%". }
+    iExists nextDiskEnd_txn_id.
+    iSplitL "HownStableSet".
+    { iExists _. iFrame. iFrame "#". iFrame "%". }
+    rewrite subslice_zero_length.
+    eapply is_txn_bound in HnextDiskEnd_txn.
+    iPureIntro. intuition eauto; lia.
+  }
+
+  iCombine "HownStableSet Hstablectx" as "Hctx".
+  iMod (map_alloc_ro with "Hctx") as "[Hctx #Hstable']"; eauto.
+  iDestruct (big_sepM_insert with "[$Hstablero Hstable']") as "Hstablero"; eauto.
+  iFrame "Hstable'".
+
+  iModIntro.
+  iDestruct "Hctx" as "[HownStableSet Hstablectx]".
+  iSplitL "Hstablectx Hstablero".
+  { iExists _. iFrame "Hstablectx". iFrame.
+    iPureIntro. eapply stable_sound_alloc. 1: apply Hstable. all: eauto. }
+
+  destruct (decide (txn_id' ≤ nextDiskEnd_txn_id)).
+  {
+    iFrame "Htxns_ctx".
+    iExists nextDiskEnd_txn_id.
+    iSplitL "HownStableSet".
+    { iExists _. iFrame. iFrame "#".
+      iPureIntro. intros.
+      destruct (decide (txn_id0 = txn_id')); try lia.
+      rewrite lookup_insert_ne; eauto. }
+    iPureIntro.
+    rewrite subslice_zero_length.
+    eapply is_txn_bound in HnextDiskEnd_txn.
+    intuition eauto; lia.
+  }
+
+  destruct (decide (nextDiskEnd_txn_id < txn_id)).
+  {
+    rewrite HnextDiskEnd_max_stable in Hstable; try lia. congruence.
+  }
+
+  assert (is_txn σ.(log_state.txns) nextDiskEnd_txn_id pos) as Hnextpos.
+  {
+    eapply (is_txn_mid _ txn_id _ txn_id'); eauto.
+    word.
+  }
+
+  pose proof (is_txn_pos_unique _ _ _ _ HnextDiskEnd_txn Hnextpos); subst.
+
+  iDestruct (txns_ctx_txn_pos _ _ txn_id' with "Htxns_ctx") as "#Htxn_id'_pos"; eauto.
+  iFrame.
+  iExists txn_id'.
+  iSplit.
+  { iExists _. iFrame. iFrame "Hstable'". iFrame "Htxn_id'_pos".
+    iPureIntro. intros. rewrite lookup_insert_ne; last by lia.
+    eapply HnextDiskEnd_max_stable. lia. }
+  eapply is_txn_bound in Histxn' as Histxn'_bound.
+  iPureIntro. intuition try lia.
+  eapply stable_sound_nils; eauto.
+Qed.
 
 End goose_lang.
