src/program_proof/wal/flush_proof.v
@@ -47,7 +47,7 @@ Proof.
   iNamed "Hdisk".
   iNamed "Hdisk".
   iNamed "circ.end".
-  pose proof (is_highest_txn_bound Hend_txn) as Hend_bound.
+  pose proof (is_txn_bound _ _ _ Hend_txn) as Hend_bound.
   iMod (fupd_intro_mask' _ (⊤ ∖ ↑N)) as "HinnerN"; first by solve_ndisj.
   iMod ("Hfupd" $! σ (set log_state.durable_lb (λ _, diskEnd_txn_id) σ)
           with "[% //] [%] [$HP]") as "[HP HQ]".
@@ -68,21 +68,27 @@ Proof.
   - simpl.
     iFrame.
     iExists _; iFrame.
-    iExists _, _; iFrame "# ∗".
-    eauto.
+    iExists installed_txn_id, _. simpl. iFrame "# ∗".
+    iExists _. iFrame "%". iPureIntro. lia.
 Qed.
 
-Theorem simulate_flush l γ Q σ pos txn_id :
+Theorem simulate_flush l γ Q σ pos txn_id nextDiskEnd_txn_id mutable :
   is_circular circN (circular_pred γ) γ.(circ_name) -∗
   (is_wal_inner l γ σ ∗ P σ) -∗
   diskEnd_at_least γ.(circ_name) (int.val pos) -∗
   txn_pos γ txn_id pos -∗
+  memLog_linv_nextDiskEnd_txn_id γ mutable nextDiskEnd_txn_id -∗
   (∀ (σ σ' : log_state.t) (b : ()),
       ⌜wal_wf σ⌝
         -∗ ⌜relation.denote (log_flush pos txn_id) σ σ' b⌝ -∗ P σ ={⊤ ∖ ↑N}=∗ P σ' ∗ Q) -∗
-  |={⊤ ∖ ↑innerN}=> (∃ σ', is_wal_inner l γ σ' ∗ P σ') ∗ Q.
+  |={⊤ ∖ ↑innerN}=>
+      ∃ σ' nextDiskEnd_txn_id',
+        is_wal_inner l γ σ' ∗ P σ' ∗ Q ∗
+        memLog_linv_nextDiskEnd_txn_id γ mutable nextDiskEnd_txn_id' ∗
+        ⌜nextDiskEnd_txn_id ≤ nextDiskEnd_txn_id' < length σ.(log_state.txns)⌝ ∗
+        ⌜Forall (λ x, x.2 = []) (subslice (S nextDiskEnd_txn_id) (S nextDiskEnd_txn_id') σ.(log_state.txns))⌝.
 Proof.
-  iIntros "#Hcirc Hinv #Hlb #Hpos_txn Hfupd".
+  iIntros "#Hcirc Hinv #Hlb #Hpos_txn HstableSet Hfupd".
   iDestruct "Hinv" as "[Hinner HP]".
   iNamed "Hinner".
   iNamed "Hdisk".
@@ -91,8 +97,8 @@ Proof.
   iMod (is_circular_diskEnd_lb_agree with "Hlb Hcirc Howncs") as "(%Hlb&Howncs)"; first by solve_ndisj.
   iDestruct (txn_pos_valid_general with "Htxns_ctx Hpos_txn") as %His_txn.
   pose proof (is_txn_bound _ _ _ His_txn).
-  pose proof (is_highest_txn_bound Hend_txn).
-  pose proof (wal_wf_txns_mono_pos Hwf His_txn (is_highest_weaken Hend_txn)).
+  pose proof (is_txn_bound _ _ _ Hend_txn).
+  pose proof (wal_wf_txns_mono_pos Hwf His_txn Hend_txn).
 
   iMod (fupd_intro_mask' _ (⊤ ∖ ↑N)) as "HinnerN"; first by solve_ndisj.
   iMod ("Hfupd" $! σ (set log_state.durable_lb (λ _, Nat.max σ.(log_state.durable_lb) txn_id) σ) with "[% //] [%] HP") as "[HP HQ]".
@@ -101,8 +107,77 @@ Proof.
     lia. }
   iMod "HinnerN" as "_".
   iFrame "HQ".
+
+  iAssert (|==> ⌜Forall (λ x, x.2 = []) (subslice (S diskEnd_txn_id) (S (diskEnd_txn_id `max` txn_id)) σ.(log_state.txns))⌝ ∗
+           (diskEnd_txn_id `max` txn_id)%nat [[γ.(stable_txn_ids_name)]]↦ro tt ∗
+           nextDiskEnd_inv γ σ.(log_state.txns) ∗
+           txns_ctx γ σ.(log_state.txns) ∗
+           ∃ nextDiskEnd_txn_id',
+             memLog_linv_nextDiskEnd_txn_id γ mutable nextDiskEnd_txn_id' ∗
+             ⌜nextDiskEnd_txn_id ≤ nextDiskEnd_txn_id' < length σ.(log_state.txns)⌝ ∗
+             ⌜Forall (λ x, x.2 = []) (subslice (S nextDiskEnd_txn_id) (S nextDiskEnd_txn_id') σ.(log_state.txns))⌝
+          )%I
+    with "[HstableSet HnextDiskEnd_inv Htxns_ctx]"
+    as "H".
+  {
+    destruct (decide (txn_id ≤ diskEnd_txn_id)).
+    { rewrite -> (max_l diskEnd_txn_id txn_id) by lia.
+      rewrite ?subslice_zero_length. iSplitR; first by done.
+
+      iAssert (⌜nextDiskEnd_txn_id < length σ.(log_state.txns)⌝)%I as "%HnextDiskEnd_txn_bound".
+      {
+        iNamed "HstableSet".
+        iDestruct (txn_pos_valid_general with "Htxns_ctx HnextDiskEnd_txn") as %HnextDiskEnd_txn_bound.
+        eapply is_txn_bound in HnextDiskEnd_txn_bound. iPureIntro. lia.
+      }
+
+      iFrame "Hend_txn_stable".
+      iFrame "HnextDiskEnd_inv".
+      iFrame "Htxns_ctx".
+      iExists nextDiskEnd_txn_id.
+      rewrite ?subslice_zero_length.
+      iFrame "HstableSet".
+      iModIntro. iPureIntro. intuition eauto; try lia.
+    }
+
+    pose proof (wal_wf_txns_mono_pos Hwf His_txn Hend_txn).
+    rewrite -> max_r by lia.
+    replace diskEnd with pos in * by word.
+
+    iMod (stable_txn_id_advance _ _ _ txn_id
+          with "HstableSet HnextDiskEnd_inv Hend_txn_stable Htxns_ctx")
+      as "H"; eauto.
+    { lia. }
+
+    iDestruct "H" as "(Hstable & HnextDiskEnd_inv & Htxns_ctx & H)".
+    iDestruct "H" as (nextDiskEnd_txn_id') "(HstableSet & %Hle & %Hnils')".
+    iModIntro.
+
+    iSplit.
+    {
+      iDestruct (subslice_stable_nils with "[$HnextDiskEnd_inv $Hend_txn_stable]") as "H".
+      1: eassumption.
+      2: eassumption.
+      2: eapply His_txn.
+      1: lia.
+      done.
+    }
+
+    iFrame "Hstable".
+    iFrame "HnextDiskEnd_inv".
+    iFrame "Htxns_ctx".
+    iExists nextDiskEnd_txn_id'.
+    iFrame "HstableSet".
+    done.
+  }
+
+  iMod "H" as "(%Hnils & #Hstable & HnextDiskEnd_inv & Htxns_ctx & H)".
+  iDestruct "H" as (nextDiskEnd_txn_id') "(HstableSet & %Hle & %Hnils')".
+
   iModIntro.
-  iExists _; iFrame "HP".
+  iExists _, nextDiskEnd_txn_id'; iFrame "HP".
+  iFrame "HstableSet".
+  iFrame "%".
   iSplit; auto.
   { iPureIntro.
     eapply wal_wf_update_durable; eauto.
@@ -111,22 +186,28 @@ Proof.
   }
   simpl.
   iFrame.
-  assert (txn_id ≤ diskEnd_txn_id)%nat.
-  { destruct (decide (pos = diskEnd)); subst.
-    - apply Hend_txn in His_txn; lia.
-    - assert (int.val pos ≠ int.val diskEnd).
-      { intros ?.
-        apply n.
-        word. }
-      lia.
-  }
   iExists _; iFrame.
-  iExists installed_txn_id, diskEnd_txn_id; iFrame "# ∗".
-  iExists diskEnd.
-  iPureIntro.
-  split_and!; simpl; auto.
-  cut (txn_id ≤ diskEnd_txn_id)%nat; first by lia.
-  lia.
+  iExists installed_txn_id, (Nat.max diskEnd_txn_id txn_id). iFrame "# ∗".
+  iSplitL "Hinstalled".
+  { iNamed "Hinstalled". iExists _, _. iFrame. iPureIntro. intuition try lia.
+    eapply Nat.max_lub_lt; eauto. }
+  iSplit.
+  - iDestruct "Hdurable" as %Hcirc_matches. iPureIntro. simpl.
+    unfold circ_matches_txns in *. intuition try lia.
+    rewrite -> (subslice_split_r _ (S diskEnd_txn_id) _ σ.(log_state.txns)) by lia.
+    eapply has_updates_app_nils; eauto.
+  - iExists diskEnd.
+    iPureIntro.
+    split_and!; simpl; auto.
+    + eapply Nat.max_le_compat_r. lia.
+    + pose proof (wal_wf_txns_mono_pos Hwf His_txn Hend_txn).
+      destruct (decide (txn_id ≤ diskEnd_txn_id)).
+      { rewrite max_l; last by lia. eauto. }
+      rewrite max_r; last by lia.
+      destruct (decide (int.val pos = int.val diskEnd)); try lia.
+      replace diskEnd with pos; eauto.
+      word.
+
   Unshelve.
   all: try constructor.
 Qed.
@@ -226,12 +307,38 @@ Proof.
   iInv "Hwal" as "Hinv".
   wp_call.
   iDestruct "Hinv" as (σ) "[Hinner HP]".
-  iMod (simulate_flush with "[$] [$Hinner $HP] HdiskEnd_lb Hpos_txn Hfupd") as "[Hinv HQ]".
+  iNamed "Hlkinv".
+  iNamed "HmemLog_linv".
+
+  iAssert (⌜txns = σ.(log_state.txns)⌝)%I as "%Htxnseq".
+  {
+    iNamed "Hinner".
+    iDestruct (ghost_var_agree with "Howntxns γtxns") as "%Htxnseq".
+    done.
+  }
+  subst.
+
+  iMod (simulate_flush with "Hcirc [$Hinner $HP] HdiskEnd_lb Hpos_txn HnextDiskEnd Hfupd") as "H".
+  iDestruct "H" as (σ' nextDiskEnd_txn_id') "(Hinner & HP & HQ & HnextDiskEnd & %Hle & %Hnils)".
   iModIntro.
-  iFrame "Hinv".
+
+  iSplitL "Hinner HP".
+  { iNext. iExists _. iFrame. }
 
   wp_loadField.
-  wp_apply (release_spec with "[$lk $Hlocked $Hlkinv]").
+  wp_apply (release_spec with "[-HQ HΦ]").
+  { iFrame "lk". iFrame "Hlocked". iNext. iExists _.
+    iFrame.
+    iExists _, _, _, _.
+    iFrame. iFrame "#". iFrame "%".
+    iPureIntro. intuition try lia.
+    - rewrite <- (subslice_to_end _ (length σ.(log_state.txns)) σ.(log_state.txns)) by lia.
+      rewrite <- (subslice_to_end _ (length σ.(log_state.txns)) σ.(log_state.txns)) in His_nextTxn by lia.
+      rewrite -> (subslice_split_r _ (S nextDiskEnd_txn_id') _ σ.(log_state.txns)) in His_nextTxn by lia.
+      eapply has_updates_prepend_nils in His_nextTxn; eauto.
+    - rewrite -> (subslice_split_r _ (S nextDiskEnd_txn_id) _ σ.(log_state.txns)); try lia.
+      eapply has_updates_app_nils; eauto.
+  }
   iApply ("HΦ" with "HQ").
 Qed.
 
